Start putting together pure_to_thunk pass

compiler/backend/passes/proofs/pure_to_thunkProofScript.sml
@@ -73,6 +73,7 @@ Inductive exp_rel:
        exp_rel (App i f xs) (Apps g (MAP Delay ys))) ∧
 [~Case:]
   (∀i x v xs ys.
+     ~MEM v (FLAT (MAP (FST ∘ SND) xs)) ∧ xs ≠ [] ∧
      MAP FST xs = MAP FST ys ∧
      MAP (FST o SND) xs = MAP (FST o SND) ys ∧
      LIST_REL exp_rel (MAP (SND o SND) xs) (MAP (SND o SND) ys) ⇒
@@ -83,26 +84,110 @@ Inductive exp_rel:
 End
 
 Overload to_thunk = “pure_to_thunk_1Proof$compile_rel”
-Overload lift_rel = “thunk_case_liftProof$exp_rel”
+Overload lift_rel = “thunk_case_liftProof$compile_rel”
 Overload d2b_rel = “thunk_case_d2bProof$exp_rel”
+
+Theorem LIST_REL_combined_IMP:
+  ∀xs ys.
+    LIST_REL (λx y.
+      exp_rel x y ∧
+      ∃y1 y2. to_thunk (exp_of x) y1 ∧ lift_rel y1 y2 ∧ d2b_rel y2 y) xs ys ⇒
+    ∃ts1 ts2.
+      LIST_REL (λx y. to_thunk (exp_of x) y) xs ts1 ∧
+      LIST_REL lift_rel ts1 ts2 ∧
+      LIST_REL d2b_rel ts2 ys
+Proof
+  Induct \\ Cases_on ‘ys’ \\ fs [] \\ rw []
+  \\ first_x_assum drule \\ fs [] \\ rw [PULL_EXISTS]
+  \\ metis_tac []
+QED
+
+Theorem to_thunk_Apps:
+  ∀xs ys x y.
+    to_thunk x y ∧ LIST_REL to_thunk xs ys ⇒
+    to_thunk (Apps x xs) (Apps y (MAP Delay ys))
+Proof
+  Induct \\ Cases_on ‘ys’ \\ fs [pure_expTheory.Apps_def,Apps_def]
+  \\ rw [] \\ first_x_assum $ irule
+  \\ simp [Once pure_to_thunk_1ProofTheory.compile_rel_cases]
+QED
+
+Theorem lift_rel_Apps:
+  ∀xs ys x y.
+    lift_rel x y ∧ LIST_REL lift_rel xs ys ⇒
+    lift_rel (Apps x (MAP Delay xs)) (Apps y (MAP Delay ys))
+Proof
+  Induct \\ Cases_on ‘ys’ \\ fs [pure_expTheory.Apps_def,Apps_def]
+  \\ rw [] \\ first_x_assum $ irule \\ fs []
+  \\ irule_at Any thunk_case_liftProofTheory.compile_rel_App \\ fs []
+  \\ irule_at Any thunk_case_liftProofTheory.compile_rel_Delay \\ fs []
+QED
+
+Theorem d2b_rel_Apps:
+  ∀xs ys x y.
+    d2b_rel x y ∧ LIST_REL d2b_rel xs ys ⇒
+    d2b_rel (Apps x (MAP Delay xs)) (Apps y (MAP Delay ys))
+Proof
+  Induct \\ Cases_on ‘ys’ \\ fs [pure_expTheory.Apps_def,Apps_def]
+  \\ rw [] \\ first_x_assum $ irule \\ fs []
+  \\ irule_at Any thunk_case_d2bProofTheory.exp_rel_App \\ fs []
+  \\ irule_at Any thunk_case_d2bProofTheory.exp_rel_Delay \\ fs []
+QED
 
 Theorem exp_rel_imp_combined:
   ∀x y.
     exp_rel x y ⇒
-    ∃y1 y2 y3.
+    ∃y1 y2.
       to_thunk (exp_of x) y1 ∧
-      lift_rel y2 y3 ∧
-      d2b_rel y3 y
+      lift_rel y1 y2 ∧
+      d2b_rel y2 y
 Proof
-  cheat
+
+  Induct_on ‘exp_rel’ \\ rw [pureLangTheory.exp_of_def]
+  >~ [‘Var n’] >-
+   (simp [Once pure_to_thunk_1ProofTheory.compile_rel_cases]
+    \\ irule_at Any thunk_case_liftProofTheory.compile_rel_Force
+    \\ irule_at Any thunk_case_d2bProofTheory.exp_rel_Force
+    \\ irule_at Any thunk_case_d2bProofTheory.exp_rel_Var
+    \\ irule_at Any thunk_case_liftProofTheory.compile_rel_Var)
+  >~ [‘Lams s’] >-
+   (qid_spec_tac ‘s’ \\ Induct
+    \\ fs [Lams_def,pure_expTheory.Lams_def]
+    >- metis_tac []
+    \\ rw []
+    \\ irule_at Any thunk_case_liftProofTheory.compile_rel_Lam
+    \\ irule_at Any thunk_case_d2bProofTheory.exp_rel_Lam
+    \\ first_x_assum $ irule_at Any
+    \\ first_x_assum $ irule_at Any
+    \\ simp [Once pure_to_thunk_1ProofTheory.compile_rel_cases])
+  >~ [‘Let’] >-
+   (irule_at Any pure_to_thunk_1ProofTheory.compile_rel__Let
+    \\ first_x_assum $ irule_at $ Pos hd
+    \\ first_x_assum $ irule_at $ Pos hd
+    \\ irule_at Any thunk_case_liftProofTheory.compile_rel_Let
+    \\ irule_at Any thunk_case_liftProofTheory.compile_rel_Delay
+    \\ first_x_assum $ irule_at $ Pos hd
+    \\ first_x_assum $ irule_at $ Pos hd
+    \\ irule_at Any thunk_case_d2bProofTheory.exp_rel_Let
+    \\ irule_at Any thunk_case_d2bProofTheory.exp_rel_Delay \\ fs [])
+  >~ [‘Apps’] >-
+   (drule LIST_REL_combined_IMP \\ strip_tac
+    \\ qexists_tac ‘Apps y1 (MAP Delay ts1)’
+    \\ qexists_tac ‘Apps y2 (MAP Delay ts2)’
+    \\ irule_at Any to_thunk_Apps \\ simp [listTheory.LIST_REL_MAP1]
+    \\ fs [combinTheory.o_DEF,SF ETA_ss]
+    \\ irule_at Any lift_rel_Apps \\ fs []
+    \\ irule_at Any d2b_rel_Apps \\ fs [])
+  >~ [‘rows_of’] (* i.e. Case *)
+
+  \\ cheat
 QED
 
 (*
 
 TODO:
- - remove closed from Letrec and Seq in pure_to_thunk_1Proof
- - add Let case to pure_to_thunk_1Proof
- - remove ticks from thunk_case_liftProof
+ - remove closed from Letrec in pure_to_thunk_1Proof
+ - make thunk_case_inl usable
 
 *)
 
